theories/Decidability.v
@@ -4,12 +4,9 @@ From LogRel.AutoSubst Require Import core unscoped Ast Extra.
 From LogRel Require Import Utils BasicAst Context Notations UntypedReduction DeclarativeTyping DeclarativeInstance GenericTyping NormalForms.
 From LogRel Require Import AlgorithmicTyping BundledAlgorithmicTyping AlgorithmicConvProperties AlgorithmicTypingProperties.
 From LogRel.Decidability Require Import Functions Soundness Completeness Termination.
-From PartialFun Require Import Monad PartialFun.
+From PartialFun Require Import Monad PartialFun Exception.
 
 Import AlgorithmicTypingData DeclarativeTypingProperties.
-Import IndexedDefinitions.
-
-#[local]Existing Instance ty_errors.
 
 Definition inspect {A} (a : A) : {b | a = b} :=
   exist _ a eq_refl.
@@ -23,8 +20,8 @@ Equations check (Γ : context) (t T : term) (hΓ : [|- Γ]) (hT : [Γ |- T]) :
 
 check Γ t T hΓ hT with (inspect (def typing (check_state;Γ;T;t) _)) :=
   {
-    | ok _ eqn: e => inl _
-    | error _ eqn: e => inr _
+    | success _ eqn: e => inl _
+    | exception _ eqn: e => inr _
   }.
 Next Obligation.
   intros.
@@ -45,11 +42,10 @@ Next Obligation.
   set (Hter := check_obligations_obligation_1 _ _ _ _ _) in *.
   clearbody Hter.
   pose proof (def_graph_sound _ _ Hter) as Hgraph.
-  enough (graph typing (check_state;Γ;T;t) (ok tt)).
+  enough (graph typing (check_state;Γ;T;t) ok).
   {
     eapply orec_graph_functional in Hgraph ; tea.
-    assert (ok tt = error e0) by (etransitivity ; eassumption).
-    now congruence.
+    assert (ok = exception e0) as [=] by (etransitivity ; eassumption).
   }
   eapply algo_typing_complete in Hty as [].
   apply typing_complete.
